fairneris/examples/retransmit_example.v
@@ -1,0 +1,241 @@
+From stdpp Require Import list fin_maps.
+From iris.proofmode Require Import proofmode.
+From trillium.program_logic Require Import ectx_lifting.
+From fairneris Require Import fairness.
+From fairneris.examples Require Import retransmit_model_progress_ltl.
+From fairneris.aneris_lang Require Import aneris_lang.
+From fairneris.aneris_lang.state_interp Require Import state_interp state_interp_events.
+From fairneris.aneris_lang.program_logic Require Import aneris_weakestpre.
+(* From fairneris Require Import adequacy. *)
+
+Definition Aprog shA : expr := SendToRepeat #(LitSocket shA) #"Hello" #saB.
+Definition Bprog shB : expr := ReceiveFrom #(LitSocket shB).
+
+Section with_Σ.
+  Context `{anerisG retransmit_fair_model Σ}.
+
+  Lemma wp_A s E shA :
+    {{{ shA ↪[ip_of_address saA] sA ∗ saA ⤳ (∅,∅) ∗ saB ⤇ (λ _, True) ∗
+        live_role_frag_own Arole }}}
+      (mkExpr (ip_of_address saA) (Aprog shA)) @ s; (ip_of_address saA,tidA); E
+    {{{ v, RET v; dead_role_frag_own Arole }}}.
+  Proof.
+    iIntros (Φ) "(Hsh & Hrt & #Hmsg & HA) HΦ".
+    iAssert (∃ R T, saA ⤳ (R, T) ∗
+            [∗ set] m ∈ R, socket_address_group_own {[m_sender m]})%I
+      with "[Hrt]" as (R T) "[HRT HR]"; [by eauto|].
+    iLöb as "IH" forall (R T).
+    iApply wp_lift_head_step_fupd; [done|].
+    iIntros (ex atr K tp1 tp2 σ Hexvalid Hex Hlocale)
+            "(%Hvalid & Hσ & [Hlive_auth Hlive_owns] & Hauth) /=".
+    iMod (steps_auth_update_S with "Hauth") as "Hauth".
+    rewrite (last_eq_trace_ends_in _ _ Hex).
+    iDestruct (aneris_state_interp_socket_valid with "Hσ Hsh")
+      as (Sn r) "[%HSn (%Hr & %Hreset)]".
+    iApply fupd_mask_intro; [set_solver|]. iIntros "Hclose".
+    iSplitR.
+    { iPureIntro; do 4 eexists. eapply SocketStepS; eauto. by econstructor. }
+    iIntros (α ? ? ? Hstep). simpl in *. iModIntro. inv_head_step; iNext.
+    rewrite (insert_id (state_sockets σ)); last done.
+    iAssert (socket_address_group_own {[saA]})%I as "#HsaA".
+    { iDestruct "HRT" as "[(%send & %recv & _ & _ & _ & $ & _) _]". }
+    iAssert (socket_address_group_own {[saB]})%I as "#HsaB".
+    { by iDestruct "Hmsg" as (γ) "[H _]". }
+    iMod (aneris_state_interp_send shA saA {[saA]} saB {[saB]} _ _ sA _ _ _ _ _
+                                   "Hello"
+           with "[$HsaA] [$HsaB] [$Hsh] [HRT] [$Hmsg] [] [$Hσ]")
+        as "(%Hmhe & Hσ & Hsh & HRT)";
+      [try set_solver..|].
+    { apply message_group_equiv_refl; set_solver. }
+    { iDestruct "HRT" as "[$ _]". }
+    { by rewrite /from_singleton; eauto. }
+    iDestruct (live_role_auth_elem_of with "Hlive_auth HA") as %Hrole.
+    destruct (trace_last atr) as [[st ms] bs] eqn:Heqn.
+    iExists (st,ms ⊎ {[ (mkMessage saA saB "Hello") ]},bs),
+              (inl (Arole,Some (mkMessage saA saB "Hello"))).
+    iMod "Hclose". rewrite -Hmhe. iFrame=> /=.
+    iSplitR; last first.
+    { iDestruct "HR" as "#HR".
+      iApply ("IH" with "Hsh HA HΦ [HRT]"); [by iSplitL|done]. }
+    iPureIntro.
+    rewrite /simple_valid_state_evolution in Hvalid.
+    rewrite /simple_valid_state_evolution=> /=.
+    destruct Hvalid as (Hsteps & Hmatch & Hlive & Hms & Hskt).
+    rewrite /trace_ends_in in Hex.
+    rewrite Hex in Hms. simpl in Hms. rewrite Hms.
+    split; [econstructor; [done|econstructor|done]|].
+    split; [done|].
+    split.
+    { intros ℓ ζ Hlabels Henabled=> /=. rewrite right_id_L.
+      rewrite Hex in Hlive. eapply Hlive; [done|by rewrite Heqn]. }
+    split; last first.
+    { simpl. rewrite Hex in Hskt. simpl in *. by rewrite Heqn in Hskt. }
+    simpl. rewrite Heqn in Hms. simpl in *.
+    rewrite Heqn. simpl. multiset_solver.
+  Qed.
+
+  Lemma wp_B s E shB :
+    {{{ shB ↪[ip_of_address saB] sB ∗ saB ⤳ (∅,∅) ∗ saB ⤇ (λ _, True) ∗
+        live_role_frag_own Brole }}}
+      (mkExpr (ip_of_address saB) (Bprog shB)) @ s; (ip_of_address saB, tidB); E
+    {{{ v, RET v; dead_role_frag_own Brole }}}.
+  Proof.
+    iIntros (Φ) "(Hsh & Hrt & #HΨ & HB) HΦ".
+    iLöb as "IH".
+    iApply wp_lift_head_step; auto.
+    iIntros (ex atr K tp1 tp2 σ Hexvalid Hex) "(%Hvalid & Hσ & [Hlive_auth Hdead_auth] & Hauth) /=".
+    iMod (steps_auth_update_S with "Hauth") as "Hauth".
+    rewrite (last_eq_trace_ends_in _ _ Hex).
+    iDestruct (aneris_state_interp_network_sockets_coh_valid with "Hσ") as %Hcoh.
+    iDestruct (aneris_state_interp_socket_valid with "Hσ Hsh")
+      as (Sn r) "[%HSn (%Hr & %Hreset)]".
+    iDestruct (live_role_auth_elem_of with "Hlive_auth HB") as %Hrole.
+    destruct (trace_last atr) as [[[] ms] bs] eqn:Heqn; last first.
+    { rewrite Heqn in Hrole. set_solver. }
+    simpl in *.
+    destruct Hvalid as (Hsteps & Hmatch & Hlive & [Hms Hskts]).
+    rewrite Hex in Hskts. rewrite Heqn in Hskts.
+    simpl in *.
+    subst.
+    assert (bs !! saB = Some r) as Hbs.
+    { by eapply Hskts. }
+    destruct (decide (r = [])) as [-> | Hneq].
+    - iMod (fupd_mask_intro_subseteq _ ∅ True%I with "[]") as "Hmk";
+        first set_solver; auto.
+      iModIntro. iSplitR.
+      { by iPureIntro; do 4 eexists; eapply SocketStepS; eauto; econstructor. }
+      iIntros (v2' ? ? ? Hstep).
+      inv_head_step.
+      { assert (length (r ++ [m]) = length ([] : list message))
+          as Hdone; [by f_equal|].
+        rewrite app_length /= in Hdone. lia. }
+      rewrite (insert_id (state_sockets σ)); last done.
+      iNext.
+      iMod "Hmk" as "_".
+      iModIntro.
+      iExists (retransmit_model_base.Start, ms, bs), (inl (Brole, None)).
+      rewrite -message_history_evolution_id.
+      rewrite Heqn.
+      iFrame.
+      iSplitR; last first.
+      { iSplitL; [|done]. by iApply ("IH" with "Hsh Hrt HB HΦ"). }
+      iPureIntro.
+      rewrite /trace_ends_in in Hex.
+      rewrite /trace_ends_in in Hex.
+      split; [econstructor;[done|econstructor|done]|].
+      { rewrite lookup_total_alt. by rewrite Hbs. }
+      rewrite Hex in Hms. rewrite Heqn in Hms.
+      split; [done|].
+      split; [|done].
+      intros ℓ ζ Hlabels Henabled.
+      rewrite right_id_L.
+      rewrite Hex in Hlive. eapply Hlive; [done|by rewrite Heqn].
+    - iMod (fupd_mask_intro_subseteq _ ∅ True%I with "[]") as "Hmk";
+        first set_solver; auto.
+      iModIntro. iSplitR.
+      { iPureIntro. apply last_is_Some in Hneq as [m Hneq].
+        apply last_Some in Hneq as [? ->].
+        do 4 eexists; eapply SocketStepS; eauto; econstructor; eauto 2. }
+      iIntros (v2' ? ? ? Hstep).
+      inv_head_step.
+      iNext.
+      iMod "Hmk" as "_".
+      iAssert (socket_address_group_own {[saB]})%I as "#HsaB".
+      { iDestruct "Hrt" as "[(%send & %recv & _ & _ & _ & $ & _) _]". }
+
+      iPoseProof (aneris_state_interp_receive_some saB {[saB]} _ _ _ _ (Some _)
+                   with "[] [$HΨ] [$Hσ] [$Hsh] [Hrt]")
+        as (R' sagT) "(%HinT & #HownT & %Hhist & %HR & Hrt & Hrest)";
+        [by set_solver..| | |].
+      { iFrame "#". iPureIntro. set_solver. }
+      { iDestruct "Hrt" as "[$ Hrt]". }
+      iMod "Hrest" as "(Hσ & Hsh & Ha)".
+      iMod (live_roles_auth_delete with "Hlive_auth HB") as "Hlive_auth".
+      iMod (dead_role_auth_extend _ (Brole : fmrole retransmit_fair_model) with "Hdead_auth")
+        as "[Hdead_auth Hdead_own]"; [by set_solver|].
+      iModIntro.
+      iExists (retransmit_model_base.Received, ms, <[saB:=r0]>bs),
+                (inl (Brole, None)).
+      rewrite Heqn Hhist=> /=.
+      rewrite /thread_live_roles_interp /retransmit_live_roles. simpl in *.
+      replace ({[Arole; Brole]} ∖ {[Brole]}) with ({[Arole]} : gset _)
+                                                  by set_solver.
+      replace({[Brole]} ∪ all_roles ∖ {[Arole; Brole]}) with
+        (all_roles ∖ {[Arole]} : gset _) by set_solver.
+      rewrite !right_id_L.
+      iFrame "Hauth Hlive_auth Hdead_auth Hσ".
+      iSplitR "HΦ Hdead_own"; last first.
+      { iSplit; [|done]. iApply wp_value. by iApply "HΦ". }
+      iPureIntro.
+      split; [econstructor;[done|econstructor|done]|].
+      { rewrite lookup_total_alt. by rewrite Hbs. }
+      rewrite Hex in Hms. rewrite Heqn in Hms.
+      split; [done|].
+      split; last first.
+      { split; [done|]. by eapply state_buffers_delete. }
+      intros [ℓ α] ζ Hlabels Henabled.
+      rewrite Hex in Hlive. rewrite Heqn in Hlive. simpl.
+      assert (ℓ = Arole).
+      { rewrite /role_enabled_model in Henabled. simpl in *.
+        rewrite /retransmit_live_roles in Henabled. simpl in *.
+        set_solver. }
+      simplify_eq.
+      eapply from_locale_step; last first.
+      { eapply Hlive; [done|].
+        rewrite /role_enabled_model.
+        set_solver. }
+      eapply locale_step_atomic; eauto.
+      { f_equiv; [|done].
+        f_equiv. f_equiv. apply app_nil_end. }
+      repeat econstructor; set_solver.
+  Qed.
+
+End with_Σ.
+
+(* Definition initial_state shA shB := *)
+(*   ([mkExpr ipA (Aprog shA); mkExpr ipB (Bprog shB)], *)
+(*      {| state_heaps := {[ipA:=∅; ipB:=∅]}; *)
+(*        state_sockets := {[ipA := {[shA := (sA, [])]}; *)
+(*                           ipB := {[shB := (sB, [])]}]}; *)
+(*        state_ms := ∅; |}). *)
+
+(* Lemma no_drop_dup_continued_simulation shA shB : *)
+(*   fairly_terminating (initial_state shA shB). *)
+(* Proof. *)
+(*   assert (anerisPreG simple_fair_model (anerisΣ simple_fair_model)) as HPreG. *)
+(*   { apply _. } *)
+(*   eapply (simulation_adequacy_fair_termination_multiple _ _ _ _ _ {[saA;saB]}); *)
+(*     [simpl; lia| |set_solver|set_solver| |set_solver|set_solver|..| |]=> /=. *)
+(*   { intros ℓ ζ Hmatch Henabled. rewrite /role_enabled_model in Henabled. simpl. *)
+(*     assert (ℓ = A_role ∨ ℓ = B_role) as [Heq|Heq] by set_solver; simplify_eq. *)
+(*     - assert (ζ = ("0.0.0.0", 0%nat)) as ->. *)
+(*       { rewrite /labels_match /locale_simple_label in Hmatch. *)
+(*         by repeat case_match; simplify_eq. } *)
+(*       eexists _. simpl. done. *)
+(*     - assert (ζ = ("0.0.0.1", 0%nat)) as ->. *)
+(*       { rewrite /labels_match /locale_simple_label in Hmatch. *)
+(*         by repeat case_match; simplify_eq. } *)
+(*       eexists _. simpl. done. } *)
+(*   { iIntros (Hinv) "!> Hunallocated Hrt Hlive Hdead Hfree Hnode Hlbl Hsendevs Hrecvevs". *)
+(*     iIntros "Hsend_obs Hrecv_obs". *)
+(*     iIntros "!>". *)
+(*     iDestruct (unallocated_split with "Hunallocated") as "[HA HB]"; [set_solver|]. *)
+(*     rewrite big_sepS_union; [|set_solver]. *)
+(*     iDestruct "Hrt" as "[HrtA HrtB]". *)
+(*     rewrite !big_sepS_singleton. *)
+(*     rewrite /simple_live_roles=> /=. *)
+(*     replace ({[A_role; B_role]} ∖ config_roles) with (({[A_role; B_role]}):gset _) *)
+(*                                                      by set_solver. *)
+(*     iDestruct (live_roles_own_split with "Hlive") as "[HliveA HliveB]"; *)
+(*       [set_solver|]. *)
+(*     iSplitL "HrtA". *)
+(*     { iApply (wp_A with "[HrtA]"); [admit|]. *)
+(*       iIntros "!>" (v) "H". *)
+(*       iExists _. by iFrame. } *)
+(*     iSplitL "HrtB". *)
+(*     { iApply (wp_B with "[HrtB]"); [admit|]. *)
+(*       iIntros "!>" (v) "H". *)
+(*       iExists _. by iFrame. } *)
+(*     done. } *)
+(*   (* Needs to simplify requirements on initial node in Aneris adequacy *) *)
+(* Admitted. *)
